\documentclass{article}
\usepackage[affil-it]{authblk}
\usepackage{graphicx}
\usepackage[space]{grffile}
\usepackage{latexsym}
\usepackage{textcomp}
\usepackage{longtable}
\usepackage{multirow,booktabs}
\usepackage{amsfonts,amsmath,amssymb}
\usepackage{natbib}
\usepackage{url}
\usepackage{hyperref}
\hypersetup{colorlinks=false,pdfborder={0 0 0}}
% You can conditionalize code for latexml or normal latex using this.
\newif\iflatexml\latexmlfalse
\providecommand{\tightlist}{\setlength{\itemsep}{0pt}\setlength{\parskip}{0pt}}%

\usepackage[utf8]{inputenc}
\usepackage[english]{babel}




\begin{document}

\title{Modular operator and Holevo's commutation operator}


 \author{Masaki Sohma
\\
Tamagawa University, Tokyo, Japan}


\date{\today}

\bibliographystyle{plain}

\maketitle




\section{Introduction}
This paper reviews results about a modular operator \cite{Longo_1978} and a Holevo's commutation operator \cite{Holevo_1977} in the simplest case.
We mainly deal with the von Neumann algebra $\mathfrak{N}=M_n(\mathbb{C})$, 
which is the ensemble of bounded linear operators on 
the Hilbert space $\mathfrak{H}=\mathbb{C}^n$ with the inner product $(x,y)=\bar{x}^Ty$. 

Let $\rho$ be a non-degenerated density operator and 
$\omega$ be the corresponding normal state given by $\omega(A)=\mbox{Tr}\rho A$.
Considering an inner product on $\mathfrak{N}$

\begin{equation}
\label{innerP}
\langle A, B \rangle =\frac{1}{2}\omega(BA^{\ast}+A^{\ast}B),
\end{equation}
and a bilinear form on $\mathfrak{N}$
\begin{equation}
[A,B]=i\omega(A^{\ast}B-BA^{\ast}),
\end{equation}
we introduce an operator $\mathfrak{D}$ by 
\begin{equation}\label{commutation opr}
[A,X]=\langle A, \mathfrak{D}X\rangle.
\end{equation}
The operator $\mathfrak{D}$, called a commutation operator, plays an important role in the quantum estimation theory.

We regard $\mathfrak{N}$ as a Hilbert-Schmidt space with the inner product
$$
\langle A, B \rangle_2 =\mbox{Tr}(A^{\ast}B),
$$
and denote it by $\mathfrak{H}_2$.
Let us consider a $\ast$-representation on $\mathfrak{H}_2$
\begin{equation}\label{star-rep}
\ell :\mathfrak{N}\to \mathfrak{B}(\mathfrak{H}_2),
\end{equation}
where $\mathfrak{B}(\mathfrak{H}_2)$ is the ensemble of bounded operators on $\mathfrak{H}_2$
and $\ell(A)B=AB$.
Then the state $\omega$ can be written by the inner product $\langle \cdot, \cdot\rangle_2$ as 
$$
\omega(A)=\mbox{Tr}(\rho^{1/2}A\rho^{1/2})=\langle \rho^{1/2},\ell(A)\rho^{1/2}\rangle_2 .
$$
Now we can define the modular operator $\Delta$ for the von Neumann algebra $\mathfrak{M}=\ell(\mathfrak{N})$ and its cyclic separating vector $\rho^{1/2}$. 
We see such derived modular operator is related to the commutation operator
as
$$
    \Delta=\left(1+\frac{i}{2}\mathfrak{D}\right)\left(1-\frac{i}{2}\mathfrak{D}\right)^{-1}.
$$


\section{Representation on $\mathfrak{H}\otimes\mathfrak{H}$}

 We identify the Hilbert-Schmidt space $\mathfrak{H}_2(=\mathfrak{N}=M_n(\mathbb{C}))$ on $\mathfrak{H}=\mathbb{C}^n$ with $\mathfrak{H}\otimes\mathfrak{H}$
by a unitary operator satisfying 
$$
v(e_je_k^T)=e_j\otimes e_k
$$
where $e_j=(\delta_{j1},\delta_{j,2},...,\delta_{j,n})^T$ with the Kronecker delta $\delta_{j,l}$. 
For $\psi=\sum_j \lambda_j e_j$ and $\phi=\sum_k \mu_k e_k$
we have
\begin{equation}
\begin{split}
v(\psi\phi^\ast)&=\sum_{j,k}\lambda_j\bar{\mu}_k v(e_je_k^T)\\
&=\sum_{j,k}\lambda_j\bar{\mu}_k e_j\otimes e_k={\psi}\otimes \overline{\phi}.
\end{split}
\end{equation}

In the $\ast$-representation (\ref{star-rep}), $\ell(A)$ is given by $\tilde{\ell}(A)=A\otimes I_n$ on $\mathfrak{H}\otimes\mathfrak{H}$.
In fact
 \begin{equation}
 \begin{split}
 v(\ell(A)e_je_k^T)&=v(Ae_je_k^T)=Ae_j\otimes e_k\\
 &= (A\otimes I_n)e_k\otimes  e_j=\tilde{\ell}(A)v(e_je_k^T),
 \end{split} 
 \end{equation}
 and hence $\ell(A)=v^{\ast}\tilde{\ell}(A)v$. 
On the other hand, $r(A):\mathfrak{N}\in X \to XA\ni\mathfrak{N}$ is 
given by $\tilde{r}(A)=I_n\otimes A^T$ on $\mathfrak{H}\otimes\mathfrak{H}$.
In fact
 \begin{equation}
 \begin{split}
 v(r(A)e_je_k^T)&=v(e_je_k^TA)=v(e_j(A^\ast e_k)^\ast)=e_j\otimes \overline{A^\ast e_k}\\
 &= e_j \otimes A^T e_k= (I_n\otimes A^T)e_j\otimes  e_k=\tilde{r}(A)v(e_je_k^T),
 \end{split} 
 \end{equation}
 and hence $r(A)=v^{\ast}\tilde{r}(A) v$. 


\section{Modular Operator}
We give a proof  of Tomita-Takesaki theory in the case of 
$\mathfrak{M}=\ell(\mathfrak{N})$ with $\mathfrak{N}=M_n(\mathbb{C})$,
where all difficulties in the theory vanish.
We have 
$\tilde{\ell}(\mathfrak{N})^\prime=\tilde{r}(\mathfrak{N})$ and $\tilde{r}(\mathfrak{N})^\prime=\tilde{\ell}(\mathfrak{N})$ for 
$
\tilde{\ell}(\mathfrak{N})=\mathfrak{N}\otimes I_n,\tilde{r}(\mathfrak{N})=I_n\otimes \mathfrak{N}
$
and hence 
\begin{equation}
\begin{split}
\mathfrak{M}^\prime&=v^\ast \tilde{\ell}(\mathfrak{N})^\prime v= v^\ast \tilde{r}(\mathfrak{N})v=r(\mathfrak{N}) \\
\mathfrak{M}^{\prime\prime}&=v^\ast \tilde{r}(\mathfrak{N})^\prime v= v^\ast \tilde{\ell}(\mathfrak{N})v=\ell(\mathfrak{N})=\mathfrak{M}.
\end{split}
\end{equation}
We use $\rho^{1/2}$ as a cyclic and separating vector;
$$
\mathfrak{H}_2=\mathfrak{M}\rho^{1/2}=\mathfrak{M}^\prime \rho^{1/2}.
$$

 Consider  anti-linear operators on $\mathfrak{H}_2$ 
\begin{equation}\label{SF}
	 \begin{split}
		 S&:\mathfrak{M}\rho^{1/2}\ni \ell(A) \rho^{1/2} \to \ell(A)^\ast\rho^{1/2}\in\mathfrak{M}\rho^{1/2},\\
		 F&:\mathfrak{M}^\prime \rho^{1/2}\ni r(A) \rho^{1/2} \to r(A)^\ast\rho^{1/2}\in \mathfrak{M}^\prime \rho^{1/2}.
	 \end{split}
\end{equation}
	Here 
	$$
	\ell(A)^\ast=v^\ast(A\otimes I_n)^\ast v=v^\ast A^\ast \otimes I_n v=\ell(A^\ast),
	$$
	and
	$$
  r(A)^\ast=v^\ast (I_n\otimes A^T)^\ast v=v^\ast I_n\otimes (A^T)^\ast v=I_n\otimes (A^\ast)^T=r(A^\ast).
	$$
	The linear operator $\Delta=FS$ on $\mathfrak{H}_2$ is called a modular operator.

For the operator $S$, we have 
	$$
    S(X)=\rho^{-1/2}X^*\rho^{1/2}.
 	$$
	In fact, putting $X=\ell(A)\rho^{1/2}=A\rho^{1/2}$,$Y=\ell(A)^\ast\rho^{1/2}=\ell(A^\ast)\rho^{1/2}=A^\ast \rho^{1/2}$,
	$$
    Y=(X\rho^{-1/2})^\ast \rho^{1/2}=\rho^{-1/2}X^\ast\rho^{1/2},
  $$
On the other hand, for the operator $F$, we have
$$
F(X)=\rho^{1/2}X^\ast \rho^{-1/2},
$$
In fact, putting $X=r(A)\rho^{1/2}=\rho^{1/2}A$,$Y=r(A)^\ast\rho^{1/2}=r(A^\ast)\rho^{1/2}= \rho^{1/2}A^\ast$,
	$$
    Y= \rho^{1/2}(\rho^{-1/2}X)^\ast=\rho^{1/2}X^\ast\rho^{-1/2}.
  $$
Thus we have
$$
\Delta(X)=FS(X)=F(\rho^{-1/2}X^*\rho^{1/2})=\rho^{1/2}(\rho^{-1/2}X^*\rho^{1/2})^\ast \rho^{-1/2}=\rho X \rho^{-1},
$$
that is, $\Delta=v^\ast(\rho \otimes ({\rho}^{-1})^T) v$.
It follows that $\Delta^\ast=v^\ast (\rho\otimes({\rho}^{-1})^T)^\ast v=\Delta$.
Since $\Delta^{-1/2}=v^\ast(\rho^{-1/2}\otimes ({\rho}^{1/2})^T) v$, 
$$
\Delta^{-1/2}(X)=\rho^{-1/2}X\rho^{1/2}
$$
and hence 
$$
S(X)=\Delta^{-1/2}(X^\ast)=\Delta^{-1/2}J(X),
$$
where $J$ is an anti-linear operator defined by $J(X)=X^\ast$.
In a similar way we have
$$
F(X)=\Delta^{1/2}J(X).
$$
In addition 
$$
J\Delta J(X)=(\rho X^\ast \rho^{-1})^\ast=\rho^{-1}X\rho=\Delta^{-1}(X).
$$

We have 
$$
\Delta^{-it}\ell(A)\Delta^{it}=\ell(\rho^{-it}A\rho^{it}).
$$
Indeed $$\Delta^{-it}\ell(A)\Delta^{it}(X)=\Delta^{-it}(A\rho^{it}X\rho^{-it})=\rho^{-it}A\rho^{it}X\rho^{-it}\rho^{it}=\rho^{-it}A\rho^{it}X$$
and 
$$
\ell(\rho^{-it}A\rho^{it})X=\rho^{-it}A\rho^{it}X.
$$
Thus we have
$$
\Delta^{-it}\mathfrak{M}\Delta^{it}=\mathfrak{M}.
$$
     Finally we have 
       $$
          J\mathfrak{M}J=\mathfrak{M}^{\prime},
       $$
			 which is obtained from
			 $$
J\ell(A)J(X)=J(AX^\ast)=(AX^\ast)^\ast=XA^\ast
			 $$
			 and
			 $$
r(A)X=XA.
			 $$
Remark that the above discussion can be easily extend to the case where 
$\mathfrak{N}=M_{m_1}(\mathbb{C})\oplus \cdots \oplus M_{m_n}(\mathbb{C})$.
The proof of Tomita-Takesaki theory for a finite dimensional von Neumann algebra is given in the Appendix.


\section{Relation between Holevo's commutation operator and modular operator}

Let us represent the modular operator defined by (\ref{commutation opr}) on $\mathfrak{H}\otimes \mathfrak{H}$
Since it holds for $A,X,Y\in \mathfrak{H}=\mathfrak{N}=\mathfrak{K}$
that 
 \begin{equation}
 \begin{split}
 [A,X]&=i\omega(A^\ast X-XA^\ast)=i\mbox{Tr}\rho(A^\ast X-XA^\ast)\\
      &=\mbox{Tr}A^\ast i(X\rho-\rho X)=\langle A, i(X\rho-\rho X)\rangle_2\\
 \langle A,Y\rangle&=\omega((YA^\ast+A^\ast Y)/2)=\mbox{Tr}\rho((YA^\ast+A^\ast Y)/2)\\
 &=\mbox{Tr}A^\ast(\rho Y+Y\rho)/2=\langle A, \rho Y+Y\rho \rangle_2,
 \end{split}
 \end{equation}
  we have
 $$
 (\rho Y+Y\rho)/2=i(X\rho-\rho X),
 $$
 which can be represented on $\mathfrak{H}\otimes \mathfrak{H}$ as
	$$
	(I_n\otimes \rho + \rho\otimes I_n)v(Y)=2i(\rho\otimes I_n -I_n\otimes \rho )v(X).
	$$
	Thus 
	$$
	v(\mathfrak{D}X)=v(Y)=2i(I_n\otimes \rho + \rho\otimes I_n)^{-1}(\rho\otimes I_n -I_n\otimes \rho )v(X),
	$$
	that is,
	$$
	\mathfrak{D}=v^\ast[ 2i(I_n\otimes \rho + \rho\otimes I_n)^{-1}(\rho\otimes I_n -I_n\otimes \rho )]v
	$$
	  Moreover
	\begin{equation}
		\begin{split}
    1+\frac{i}{2}\mathfrak{D}&=v^\ast [ 2(I_n\otimes \rho+\rho\otimes I_n)^{-1}  I_n\otimes \rho]v,\\
    1-\frac{i}{2}\mathfrak{D}&=v^\ast [ 2(I_n\otimes \rho+\rho\otimes I_n)^{-1}\rho \otimes I_n]v,\\
    1+\frac{1}{4}\mathfrak{D}^2&=v^\ast[ 4(I_n\otimes \rho+\rho\otimes I_n)^{-2}\rho \otimes \rho]v.\\

    \end{split}
	\end{equation}

	Finally	we get
		$$
    \Delta=\left(1+\frac{i}{2}\mathfrak{D}\right)\left(1-\frac{i}{2}\mathfrak{D}\right)^{-1},
		$$
		and
		$$
     \frac{i}{2}\mathfrak{D}=(1-\Delta)(1+\Delta)^{-1}
		$$



\section{Appendix}
In this section we prove the Tomita-Takesaki theorem for a finite dimensional
von Neumann algebras $\tilde{\mathfrak{N}}$ on a Hilbert space $\mathfrak{K}$.
We assume there exists a cyclic separating vector $\xi\in \mathfrak{K}$;
$\mathfrak{K}=\tilde{\mathfrak{N}}\xi=\tilde{\mathfrak{N}}^\prime\xi$.
Then we define operators $\tilde{S},\tilde{F},\tilde{\Delta}$ on $\mathfrak{K}$ as
\begin{equation}
\begin{split}
\tilde{S}&:\tilde{\mathfrak{N}}\xi\ni X\xi \to X^\ast \xi \in \tilde{\mathfrak{N}}\xi,\\
\tilde{F}&:\tilde{\mathfrak{N}}^\prime\xi\ni Y\xi \to Y^\ast \xi \in \tilde{\mathfrak{N}}^\prime\xi,\\
\tilde{\Delta}&=\tilde{F}\tilde{S}.
\end{split}
\end{equation}
The Wedderburn theorem states that a finite dimensional $C^{\ast}$ algebra is  $\ast$-isomorphic to a direct sum of simple matrix algebras. That is, there exists $\ast$-isomorphic function $\varphi$ for von Neumann algebra $\mathfrak{N}$ such that
$$
\varphi:\tilde{\mathfrak{N}}\simeq \mathfrak{N}:=M_{m_1}(\mathbb{C})\oplus \cdots \oplus M_{m_n}(\mathbb{C})
$$

Let us consider the state on $\tilde{\mathfrak{N}}$ as
$$
\omega_\xi(A)=(\xi,A\xi),\quad A\in \tilde{\mathfrak{N}},\xi\in \mathfrak{K}.
$$
Using this state we can define the state on $\mathfrak{N}$
$$
\omega(A)=\omega_\xi(\varphi^{-1}(A)),A\in \mathfrak{N}.
$$
Applying the discussion in the previous sections to the von Neumann algebra $\mathfrak{N}$ and 
$\omega$, we get
the von Neumann algebra $\mathfrak{M}=\ell (\mathfrak{N})$ on the Hilbert space 
$\mathfrak{H}_2$, the cyclic separating vector $\rho^{1/2}\in \mathfrak{H}_2$
and operators $S, F$ and $\Delta$ on $\mathfrak{H}_2$.

Then we obtain
$$
\langle \pi(A)\rho^{1/2},\pi( B)\rho^{1/2}\rangle_2=(\varphi^{-1}(A)\xi,\varphi^{-1}(B)\xi),
$$
which means
$$
U:\mathfrak{H}_2\ni\pi(A)\rho^{1/2}\to \varphi^{-1}(A)\xi\in\mathfrak{K}, \quad A\in \mathfrak{N}
$$
gives a unitary operator from $\mathfrak{H}_2$ to $\mathfrak{K}$.
This unitary operator combines $\Delta$ and $\tilde{\Delta}$ as
$$
\tilde{\Delta}=U\Delta U^{\ast},
$$
and gives the main result of Tomita-Takesaki Theory,
$$
\tilde{\Delta}^{-it}\tilde{\mathfrak{N}}\tilde{\Delta}^{it}=\tilde{\mathfrak{N}}.
$$

\bibliography{bibliography/converted_to_latex.bib%
}

\end{document}

